theories/notations.v
@@ -1,0 +1,5 @@
+From iris Require Import base_logic.lib.gen_heap.
+
+(* Store-related notations *)
+Notation "l ↦ v" := (mapsto l (DfracOwn 1) v) (at level 20).
+
